add cache class

src/BinEncoders/Env/BinLib/Bool.v
@@ -5,29 +5,30 @@ Require Import
 Set Implicit Arguments.
 
 Section BoolBinEncoder.
-  Variable E E' : Type.
-  Variable Eequiv : E -> E' -> Prop.
+  Variable cache : Cache.
+  Variable cacheAdd : CacheAdd cache nat.
 
-  Definition Bool_encode (b : bool) (e : bctx E) : bin * bctx E := (b :: nil, (fst e, 1 + snd e)).
+  Definition Bool_encode (b : bool) (ce : CacheEncode) :=
+    (b :: nil, addE ce 1).
 
-  Definition Bool_decode (b : bin) (e : bctx E') : bool * bin * bctx E':=
+  Definition Bool_decode (b : list bool) (cd : CacheDecode) :=
     match b with
-    | nil => (false, nil, e) (* bogus *)
-    | x :: xs => (x, xs, (fst e, 1 + snd e))
+    | nil => (false, nil, cd) (* bogus *)
+    | x :: xs => (x, xs, addD cd 1)
     end.
 
   Theorem Bool_encode_correct :
-    forall predicate, encode_decode_correct (bctx_equiv Eequiv) btransformer predicate Bool_encode Bool_decode.
+    forall predicate, encode_decode_correct cache btransformer predicate Bool_encode Bool_decode.
   Proof.
     unfold encode_decode_correct, Bool_encode, Bool_decode.
     intros pred env env' xenv xenv' data data' bin ext ext' Peq Ppred Penc Pdec. simpl in *.
-    inversion Penc; clear Penc; subst. simpl in *.
-    inversion Pdec; clear Pdec; inversion Peq; clear Peq; subst; intuition.
-    split; simpl; auto.
+    inversion Penc; clear Penc; subst.
+    inversion Pdec; clear Pdec; subst.
+    intuition. apply add_correct. auto.
   Qed.
 End BoolBinEncoder.
 
-Global Instance Bool_decoder E E' ctxequiv predicate
-  : decoder (bctx_equiv ctxequiv) btransformer predicate (Bool_encode (E:=E)) :=
-  { decode := @Bool_decode E';
-    decode_correct := @Bool_encode_correct _ _ _ _ }.
+Global Instance Bool_decoder cache cacheAdd predicate
+  : decoder cache btransformer predicate (@Bool_encode cache cacheAdd) :=
+  { decode := @Bool_decode cache cacheAdd;
+    decode_correct := @Bool_encode_correct _ _ _ }.
