src/BinEncoders/Env/BinLib/Core.v
@@ -3,15 +3,9 @@ Require Import
 
 Set Implicit Arguments.
 
-Definition bin := list bool.
-
-Definition btransformer : Transformer bin :=
-  {| transform := @app _;
+Definition btransformer : Transformer :=
+  {| bin := list bool;
+     transform := @app _;
      transform_id := nil;
      transform_id_pf := @app_nil_l _;
      transform_assoc := @app_assoc _ |}.
-
-Definition bctx (A : Type) := prod A nat.
-
-Definition bctx_equiv {E E'} (ctx_equiv : E -> E' -> Prop) :=
-  fun (e : bctx E) (e' : bctx E') => ctx_equiv (fst e) (fst e') /\ snd e = snd e'.
