src/BinEncoders/Env/Common/Transformer.v
@@ -1,11 +1,8 @@
 Set Implicit Arguments.
 
-Section Transformer.
-  Variable B : Type.
-
-  Class Transformer :=
-    { transform : B -> B -> B;
-      transform_id : B;
-      transform_id_pf : forall l, transform transform_id l = l;
-      transform_assoc : forall l m n, transform l (transform m n) = transform (transform l m) n }.
-End Transformer.
+Class Transformer :=
+  { bin : Type;
+    transform : bin -> bin -> bin;
+    transform_id : bin;
+    transform_id_pf : forall l, transform transform_id l = l;
+    transform_assoc : forall l m n, transform l (transform m n) = transform (transform l m) n }.
