src/BinEncoders/Env/Lib/FixList.v
@@ -9,12 +9,12 @@ Set Implicit Arguments.
 
 Section FixListEncoder.
   Variable size : nat.
-  Variable A B E E' : Type.
-  Variable Eequiv : E -> E' -> Prop.
-  Variable transformer : Transformer B.
+  Variable A : Type.
+  Variable cache : Cache.
+  Variable transformer : Transformer.
   Variable A_predicate : A -> Prop.
-  Variable A_encode : A -> E -> B * E.
-  Variable A_decoder : decoder Eequiv transformer A_predicate A_encode.
+  Variable A_encode : A -> CacheEncode -> bin * CacheEncode.
+  Variable A_decoder : decoder cache transformer A_predicate A_encode.
 
   Definition FixList := { xs : list A | length xs < exp2_nat size }.
 
@@ -32,20 +32,20 @@ Section FixListEncoder.
     FixList_getlength l = len /\
     forall x, In x (proj1_sig l) -> A_predicate x.
 
-  Fixpoint FixList_encode' (xs : list A) (env : E) : B * E :=
+  Fixpoint FixList_encode' (xs : list A) (ce : CacheEncode) : bin * CacheEncode :=
     match xs with
-    | nil => (transform_id (B:=B), env)
-    | x :: xs' => let (b1, env1) := A_encode x env in
+    | nil => (transform_id, ce)
+    | x :: xs' => let (b1, env1) := A_encode x ce in
                   let (b2, env2) := FixList_encode' xs' env1 in
                       (transform b1 b2, env2)
     end.
 
   Definition FixList_encode (l : FixList) := FixList_encode' (proj1_sig l).
 
-  Fixpoint FixList_decode' (s : nat) (b : B) (env' : E') : list A * B * E' :=
+  Fixpoint FixList_decode' (s : nat) (b : bin) (cd : CacheDecode) : list A * bin * CacheDecode :=
     match s with
-    | O => (nil, b, env')
-    | S s' => let (x1, e1) := decode b env' in
+    | O => (nil, b, cd)
+    | S s' => let (x1, e1) := decode b cd in
               let (x, b1) := x1 in
               let (x2, e2) := FixList_decode' s' b1 e1 in
               let (xs, b2) := x2 in
@@ -57,7 +57,7 @@ Section FixListEncoder.
   Proof.
     induction len; intuition eauto.
     simpl. destruct (decode bin env) as [[? ?] ?].
-    specialize (IHlen b e). destruct (FixList_decode' len b e) as [[? ?] ?]. simpl. f_equal. eauto.
+    specialize (IHlen b c). destruct (FixList_decode' len b c) as [[? ?] ?]. simpl. f_equal. eauto.
   Qed.
 
   Lemma exp2_nat_nonzero :
@@ -69,7 +69,7 @@ Section FixListEncoder.
     intro s. specialize (lt_pf s). omega.
   Qed.
 
-  Definition FixList_decode (len : nat) (b : B) (env' : E') : FixList * B * E'.
+  Definition FixList_decode (len : nat) (b : bin) (env' : CacheDecode) : FixList * bin * CacheDecode.
     refine (exist _ (fst (fst (FixList_decode' (min (pred (exp2_nat size)) len) b env'))) _,
             snd (fst (FixList_decode' len b env')),
             snd (FixList_decode' len b env')).
@@ -81,7 +81,7 @@ Section FixListEncoder.
 
   Theorem FixList_encode_correct :
     forall len,
-      encode_decode_correct Eequiv transformer (FixList_predicate len) FixList_encode (FixList_decode (nat_of_N (proj1_sig len))).
+      encode_decode_correct cache transformer (FixList_predicate len) FixList_encode (FixList_decode (nat_of_N (proj1_sig len))).
   Proof.
     unfold encode_decode_correct, FixList_predicate, FixList_encode, FixList_decode.
     intros [len len_pf] env env' xenv xenv' [l l_pf] [l' l'_pf] bin ext ext' Eeq Ppred Penc Pdec. simpl in *.
@@ -104,22 +104,25 @@ Section FixListEncoder.
     specialize (H4 a (or_introl eq_refl)).
     destruct (A_encode a env) eqn: ?.
     destruct (decode (transform bin ext) env') as [[? ?] ?] eqn: ?.
-    destruct (FixList_encode' l e) eqn: ?. inversion H0; subst; clear H0.
+    destruct (FixList_encode' l c) eqn: ?. inversion H0; subst; clear H0.
     rewrite <- transform_assoc in Heqp0.
     pose proof (decode_correct (decoder:=A_decoder) env env' _ _ Eeq H4 Heqp Heqp0); clear Eeq H4 Heqp Heqp0.
     destruct H as [? [? ?]]. subst.
-    destruct (FixList_decode' (length l) (transform b1 ext) e0) as [[? ?] ?] eqn: ?.
-    specialize (IHl b1 xenv e0 e H Heqp1 size0).
+    destruct (FixList_decode' (length l) (transform b1 ext) c0) as [[? ?] ?] eqn: ?.
+    specialize (IHl b1 xenv c0 c H Heqp1 size0).
     rewrite Heqp in IHl. simpl in *.
     assert (length l0 < exp2_nat size0) by omega.
     intuition. subst. intuition.
   Qed.
 End FixListEncoder.
 
-Global Instance FixList_decoder A B size len E E' ctxequiv transformer
+Global Instance FixList_decoder size A len cache
+       (transformer : Transformer)
        (A_predicate : A -> Prop)
-       (A_encode : A -> E -> B * E)
-       (A_decoder : decoder ctxequiv transformer A_predicate A_encode)
-  : decoder ctxequiv transformer (@FixList_predicate size _ A_predicate len) (FixList_encode transformer A_encode) :=
-  { decode := @FixList_decode size _ _ E E' _ _ _ _ _ (nat_of_N (proj1_sig len));
-    decode_correct := @FixList_encode_correct _ _ _ _ _ _ _ _ _ _ _ }.
+       (A_encode : A -> CacheEncode -> bin * CacheEncode)
+       (A_decoder : decoder cache transformer A_predicate A_encode)
+  : decoder cache transformer
+            (FixList_predicate A_predicate len)
+            (FixList_encode cache transformer A_encode) :=
+  { decode := @FixList_decode size _  _ _ _ _ _ (nat_of_N (proj1_sig len));
+    decode_correct := @FixList_encode_correct _ _ _ _ _ _ _ _ }.
