src/BinEncoders/Env/Lib/IList.v
@@ -8,21 +8,21 @@ Set Implicit Arguments.
 
 Section IListEncoder.
   Variable size : nat.
-  Variable A B E E' : Type.
-  Variable Eequiv : E -> E' -> Prop.
-  Variable transformer : Transformer B.
+  Variable A : Type.
+  Variable cache : Cache.
+  Variable transformer : Transformer.
   Variable A_predicate : A -> Prop.
-  Variable A_encode : A -> E -> B * E.
-  Variable A_decoder : decoder Eequiv transformer A_predicate A_encode.
+  Variable A_encode : A -> CacheEncode -> bin * CacheEncode.
+  Variable A_decoder : decoder cache transformer A_predicate A_encode.
 
   Definition IList := { xs : list A | length xs = size }.
 
   Definition IList_predicate (l : IList) :=
     forall x, In x (proj1_sig l) -> A_predicate x.
 
-  Fixpoint IList_encode' (xs : list A) (env : E) : B * E :=
+  Fixpoint IList_encode' (xs : list A) (env : CacheEncode) :=
     match xs with
-    | nil => (transform_id (B:=B), env)
+    | nil => (transform_id, env)
     | x :: xs' => let (b1, env1) := A_encode x env in
                   let (b2, env2) := IList_encode' xs' env1 in
                       (transform b1 b2, env2)
@@ -30,7 +30,7 @@ Section IListEncoder.
 
   Definition IList_encode (l : IList) := IList_encode' (proj1_sig l).
 
-  Fixpoint IList_decode' (s : nat) (b : B) (env' : E') : list A * B * E' :=
+  Fixpoint IList_decode' (s : nat) (b : bin) (env' : CacheDecode) :=
     match s with
     | O => (nil, b, env')
     | S s' => let (x1, e1) := decode b env' in
@@ -40,18 +40,18 @@ Section IListEncoder.
               (x :: xs, b2, e2)
     end.
 
-  Definition IList_decode (b : B) (env' : E') : IList * B * E'.
+  Definition IList_decode (b : bin) (env' : CacheDecode) : IList * bin * CacheDecode.
     refine (exist _ (fst (fst (IList_decode' size b env'))) _,
             snd (fst (IList_decode' size b env')),
             snd (IList_decode' size b env')).
     generalize dependent b. generalize dependent env'.
     induction size. intuition eauto. intuition simpl.
-    destruct (decode b env') as [[? ?] ?]. specialize (IHn e b0).
-    destruct (IList_decode' n b0 e). destruct p. simpl. eauto.
+    destruct (decode b env') as [[? ?] ?]. specialize (IHn c b0).
+    destruct (IList_decode' n b0 c). destruct p. simpl. eauto.
   Defined.
 
   Theorem IList_encode_correct :
-    encode_decode_correct Eequiv transformer IList_predicate IList_encode IList_decode.
+    encode_decode_correct cache transformer IList_predicate IList_encode IList_decode.
   Proof.
     unfold encode_decode_correct, IList_predicate, IList_encode, IList_decode.
     intros env env' xenv xenv' [l l_pf] [l' l'_pf] bin ext ext' Eeq Ppred Penc Pdec. simpl in *.
@@ -73,21 +73,22 @@ Section IListEncoder.
     specialize (Ppred a (or_introl eq_refl)).
     destruct (A_encode a env) eqn: ?.
     destruct (decode (transform bin ext) env') as [[? ?] ?] eqn: ?.
-    destruct (IList_encode' l e) eqn: ?. inversion H0; subst; clear H0.
+    destruct (IList_encode' l c) eqn: ?. inversion H0; subst; clear H0.
     rewrite <- transform_assoc in Heqp0.
     pose proof (decode_correct (decoder:=A_decoder) env env' _ _ Eeq Ppred Heqp Heqp0); clear Eeq Ppred Heqp Heqp0.
     destruct H as [? [? ?]]. subst.
-    destruct (IList_decode' (length l) (transform b1 ext) e0) as [[? ?] ?] eqn: ?.
+    destruct (IList_decode' (length l) (transform b1 ext) c0) as [[? ?] ?] eqn: ?.
     simpl in *; inversion H1; subst; clear H1.
-    specialize (IHl _ e1 _ _ _ H Heqp1 _ _ eq_refl H2).
+    specialize (IHl _ c1 _ _ _ H Heqp1 _ _ eq_refl H2).
     rewrite H2. rewrite Heqp in *. simpl in *. intuition. subst. eauto.
   Qed.
 End IListEncoder.
 
-Global Instance IList_decoder A B size E E' ctxequiv transformer
+Global Instance IList_decoder A size cache transformer
        (A_predicate : A -> Prop)
-       (A_encode : A -> E -> B * E)
-       (A_decoder : decoder ctxequiv transformer A_predicate A_encode)
-  : decoder ctxequiv transformer (@IList_predicate size _ A_predicate) (IList_encode transformer A_encode) :=
-  { decode := @IList_decode size _ _ E E' _ _ _ _ _;
-    decode_correct := @IList_encode_correct _ _ _ _ _ _ _ _ _ _ }.
+       (A_encode : A -> CacheEncode -> bin * CacheEncode)
+       (A_decoder : decoder cache transformer A_predicate A_encode)
+  : decoder cache transformer
+            (IList_predicate A_predicate) (IList_encode cache transformer A_encode) :=
+  { decode := @IList_decode size _  _ _ _ _ _;
+    decode_correct := @IList_encode_correct _ _ _ _ _ _ _ }.
